io/MIO.fst
@@ -211,18 +211,18 @@ effect MIO
   MIOwp a fl (to_hist pre post) 
   
 let static_cmd
-  (isTrusted : bool)
+  (caller : bool)
   (cmd : io_cmds)
   (arg : io_sig.args cmd) :
   MIO (io_sig.res cmd arg) IOActions
     (requires (fun h -> io_pre cmd arg h))
     (ensures (fun h (r:io_sig.res cmd arg) lt ->
-        lt == [convert_call_to_event isTrusted cmd arg r])) =
-  MIOwp?.reflect (mio_call isTrusted cmd arg)
+        lt == [convert_call_to_event caller cmd arg r])) =
+  MIOwp?.reflect (mio_call caller cmd arg)
 
-let get_trace (isTrusted:bool) : MIOwp trace GetTraceActions
+let get_trace (caller:bool) : MIOwp trace GetTraceActions
   (fun p h -> p [] h) =
-  MIOwp?.reflect (mio_call isTrusted GetTrace ())
+  MIOwp?.reflect (mio_call caller GetTrace ())
 
 // There is no hope to prove anything about ctx without a meta-theorem about F* / without a formalization of F* & Ghost.
 // val ctx_s : (fl:erased tflag) -> MIO unit fl (fun _ -> True) (fun _ _ _ -> True) 
